\textbf{Problem 1.}

Show that $u=1-2\abs{x-\frac{1}{2}}$ satisfies the weak statement
\begin{align*}
    \int_0^1 v_xu_x \dd{x} = 4v(\tfrac{1}{2})
\end{align*}

\begin{proof}
We begin by breaking the integral into two:
\begin{align*}
    \int_0^1 v_xu_x \dd{x}
    = \int_0^{\tfrac{1}{2}-\varepsilon} v_xu_x \dd{x}
    + \int_{\tfrac{1}{2}-\varepsilon}^1 v_xu_x \dd{x}
\end{align*}

Next, let us perform integration by parts on an indefinite integral:
\begin{align*}
    \int v_xu_x \dd{x} &= vu_x - \int v u_{xx} \\
    &= vu_x & \text{because $u_{xx} = 0$}
\end{align*}

Lastly, we recognise that
\begin{align*}
    u_x = \begin{cases}
    -2 & x > \tfrac{1}{2} \\
     2 & x < \tfrac{1}{2}
    \end{cases}
\end{align*}

Understanding all this and substituting in the limits, we obtain
\begin{align*}
    \int_0^1 v_xu_x \dd{x}
    &= \int_0^{\tfrac{1}{2}-\varepsilon} v_xu_x \dd{x}
    + \int_{\tfrac{1}{2}-\varepsilon}^1 v_xu_x \dd{x} \\
    &= [vu_x]_0^{\tfrac{1}{2}-\varepsilon} + [vu_x]_{\tfrac{1}{2}-\varepsilon}^1 \\
    &= 2v(\tfrac{1}{2}-\varepsilon) - v(0)u_x(0)
    + v(1)u_x(1) - (-2)v(\tfrac{1}{2}-\varepsilon) \\
    &= 4v(\tfrac{1}{2}-\varepsilon) + v(1)u_x(1) - v(0)u_x(0)
\end{align*}

And given Dirichlet boundary conditions such that $v(1) = v(0) = 0$, we have that since $\varepsilon\rightarrow0$
\begin{align*}
    \int_0^1 v_xu_x \dd{x} = 4v(\tfrac{1}{2})
\end{align*}
\end{proof}